better presentation

src/HOL/Auth/OtwayRees_Bad.thy
@@ -22,39 +22,39 @@ lemmas indicates the possibility of this attack.*}
 consts  otway   :: "event list set"
 inductive "otway"
   intros
-         (*Initial trace is empty*)
-   Nil:  "[] \<in> otway"
+   Nil: --{*The empty trace*}
+        "[] \<in> otway"
 
-         (*The spy MAY say anything he CAN say.  We do not expect him to
-           invent new nonces here, but he can also use NS1.  Common to
-           all similar protocols.*)
-   Fake: "[| evsf \<in> otway;  X \<in> synth (analz (knows Spy evsf)) |]
+   Fake: --{*The Spy may say anything he can say.  The sender field is correct,
+            but agents don't use that information.*}
+         "[| evsf \<in> otway;  X \<in> synth (analz (knows Spy evsf)) |]
           ==> Says Spy B X  # evsf \<in> otway"
 
-         (*A message that has been sent can be received by the
-           intended recipient.*)
-   Reception: "[| evsr \<in> otway;  Says A B X \<in>set evsr |]
+        
+   Reception: --{*A message that has been sent can be received by the
+                  intended recipient.*}
+	      "[| evsr \<in> otway;  Says A B X \<in>set evsr |]
                ==> Gets B X # evsr \<in> otway"
 
-         (*Alice initiates a protocol run*)
-   OR1:  "[| evs1 \<in> otway;  Nonce NA \<notin> used evs1 |]
+   OR1:  --{*Alice initiates a protocol run*}
+	 "[| evs1 \<in> otway;  Nonce NA \<notin> used evs1 |]
           ==> Says A B {|Nonce NA, Agent A, Agent B,
                          Crypt (shrK A) {|Nonce NA, Agent A, Agent B|} |}
                  # evs1 \<in> otway"
 
-         (*Bob's response to Alice's message.
-           This variant of the protocol does NOT encrypt NB.*)
-   OR2:  "[| evs2 \<in> otway;  Nonce NB \<notin> used evs2;
+   OR2:  --{*Bob's response to Alice's message.
+             This variant of the protocol does NOT encrypt NB.*}
+	 "[| evs2 \<in> otway;  Nonce NB \<notin> used evs2;
              Gets B {|Nonce NA, Agent A, Agent B, X|} \<in> set evs2 |]
           ==> Says B Server
                   {|Nonce NA, Agent A, Agent B, X, Nonce NB,
                     Crypt (shrK B) {|Nonce NA, Agent A, Agent B|}|}
                  # evs2 \<in> otway"
 
-         (*The Server receives Bob's message and checks that the three NAs
+   OR3:  --{*The Server receives Bob's message and checks that the three NAs
            match.  Then he sends a new session key to Bob with a packet for
-           forwarding to Alice.*)
-   OR3:  "[| evs3 \<in> otway;  Key KAB \<notin> used evs3;
+           forwarding to Alice.*}
+	 "[| evs3 \<in> otway;  Key KAB \<notin> used evs3;
              Gets Server
                   {|Nonce NA, Agent A, Agent B,
                     Crypt (shrK A) {|Nonce NA, Agent A, Agent B|},
@@ -67,10 +67,10 @@ inductive "otway"
                     Crypt (shrK B) {|Nonce NB, Key KAB|}|}
                  # evs3 \<in> otway"
 
-         (*Bob receives the Server's (?) message and compares the Nonces with
-	   those in the message he previously sent the Server.
-           Need B ~= Server because we allow messages to self.*)
-   OR4:  "[| evs4 \<in> otway;  B ~= Server;
+   OR4:  --{*Bob receives the Server's (?) message and compares the Nonces with
+	     those in the message he previously sent the Server.
+             Need @{term "B \<noteq> Server"} because we allow messages to self.*}
+	 "[| evs4 \<in> otway;  B \<noteq> Server;
              Says B Server {|Nonce NA, Agent A, Agent B, X', Nonce NB,
                              Crypt (shrK B) {|Nonce NA, Agent A, Agent B|}|}
                \<in> set evs4;
@@ -78,9 +78,9 @@ inductive "otway"
                \<in> set evs4 |]
           ==> Says B A {|Nonce NA, X|} # evs4 \<in> otway"
 
-         (*This message models possible leaks of session keys.  The nonces
-           identify the protocol run.*)
-   Oops: "[| evso \<in> otway;
+   Oops: --{*This message models possible leaks of session keys.  The nonces
+             identify the protocol run.*}
+	 "[| evso \<in> otway;
              Says Server B {|Nonce NA, X, Crypt (shrK B) {|Nonce NB, Key K|}|}
                \<in> set evso |]
           ==> Notes Spy {|Nonce NA, Nonce NB, Key K|} # evso \<in> otway"
@@ -91,7 +91,7 @@ declare parts.Body  [dest]
 declare analz_into_parts [dest]
 declare Fake_parts_insert_in_Un  [dest]
 
-(*A "possibility property": there are traces that reach the end*)
+text{*A "possibility property": there are traces that reach the end*}
 lemma "[| B \<noteq> Server; Key K \<notin> used [] |]
       ==> \<exists>NA. \<exists>evs \<in> otway.
             Says B A {|Nonce NA, Crypt (shrK A) {|Nonce NA, Key K|}|}
@@ -111,10 +111,7 @@ apply (erule otway.induct, auto)
 done
 
 
-(**** Inductive proofs about otway ****)
-
-
-(** For reasoning about the encrypted portion of messages **)
+subsection{*For reasoning about the encrypted portion of messages *}
 
 lemma OR2_analz_knows_Spy:
      "[| Gets B {|N, Agent A, Agent B, X|} \<in> set evs;  evs \<in> otway |]
@@ -131,20 +128,20 @@ lemma Oops_parts_knows_Spy:
       ==> K \<in> parts (knows Spy evs)"
 by blast
 
-(*Forwarding lemma: see comments in OtwayRees.thy*)
+text{*Forwarding lemma: see comments in OtwayRees.thy*}
 lemmas OR2_parts_knows_Spy =
     OR2_analz_knows_Spy [THEN analz_into_parts, standard]
 
 
-(** Theorems of the form X \<notin> parts (knows Spy evs) imply that NOBODY
-    sends messages containing X! **)
+text{*Theorems of the form @{term "X \<notin> parts (spies evs)"} imply that
+NOBODY sends messages containing X! *}
 
-(*Spy never sees a good agent's shared key!*)
+text{*Spy never sees a good agent's shared key!*}
 lemma Spy_see_shrK [simp]:
      "evs \<in> otway ==> (Key (shrK A) \<in> parts (knows Spy evs)) = (A \<in> bad)"
-apply (erule otway.induct, force,
-       drule_tac [4] OR2_parts_knows_Spy, simp_all, blast+)
-done
+by (erule otway.induct, force,
+    drule_tac [4] OR2_parts_knows_Spy, simp_all, blast+)
+
 
 lemma Spy_analz_shrK [simp]:
      "evs \<in> otway ==> (Key (shrK A) \<in> analz (knows Spy evs)) = (A \<in> bad)"
@@ -155,10 +152,10 @@ lemma Spy_see_shrK_D [dest!]:
 by (blast dest: Spy_see_shrK)
 
 
-(*** Proofs involving analz ***)
+subsection{*Proofs involving analz *}
 
-(*Describes the form of K and NA when the Server sends this message.  Also
-  for Oops case.*)
+text{*Describes the form of K and NA when the Server sends this message.  Also
+  for Oops case.*}
 lemma Says_Server_message_form:
      "[| Says Server B {|NA, X, Crypt (shrK B) {|NB, Key K|}|} \<in> set evs;
          evs \<in> otway |]
@@ -178,9 +175,9 @@ done
 ****)
 
 
-(** Session keys are not used to encrypt other session keys **)
+text{*Session keys are not used to encrypt other session keys*}
 
-(*The equality makes the induction hypothesis easier to apply*)
+text{*The equality makes the induction hypothesis easier to apply*}
 lemma analz_image_freshK [rule_format]:
  "evs \<in> otway ==>
    \<forall>K KK. KK <= -(range shrK) -->
@@ -199,8 +196,7 @@ lemma analz_insert_freshK:
 by (simp only: analz_image_freshK analz_image_freshK_simps)
 
 
-(*** The Key K uniquely identifies the Server's  message. **)
-
+text{*The Key K uniquely identifies the Server's  message. *}
 lemma unique_session_keys:
      "[| Says Server B {|NA, X, Crypt (shrK B) {|NB, K|}|}   \<in> set evs;
          Says Server B' {|NA',X',Crypt (shrK B') {|NB',K|}|} \<in> set evs;
@@ -208,14 +204,13 @@ lemma unique_session_keys:
 apply (erule rev_mp)
 apply (erule rev_mp)
 apply (erule otway.induct, simp_all)
-(*Remaining cases: OR3 and OR4*)
-apply blast+
+apply blast+  --{*OR3 and OR4*}
 done
 
 
-(** Crucial secrecy property: Spy does not see the keys sent in msg OR3
+subsection{*Crucial secrecy property: Spy does not see the keys sent in msg OR3
     Does not in itself guarantee security: an attack could violate
-    the premises, e.g. by having A=Spy **)
+    the premises, e.g. by having @{term "A=Spy"} *}
 
 lemma secrecy_lemma:
  "[| A \<notin> bad;  B \<notin> bad;  evs \<in> otway |]
@@ -228,9 +223,9 @@ apply (erule otway.induct, force)
 apply (frule_tac [7] Says_Server_message_form)
 apply (drule_tac [6] OR4_analz_knows_Spy)
 apply (drule_tac [4] OR2_analz_knows_Spy)
-apply (simp_all add: analz_insert_eq analz_insert_freshK pushes, spy_analz)  (*Fake*)
-(*OR3, OR4, Oops*)
-apply (blast dest: unique_session_keys)+
+apply (simp_all add: analz_insert_eq analz_insert_freshK pushes)
+apply spy_analz  --{*Fake*}
+apply (blast dest: unique_session_keys)+  --{*OR3, OR4, Oops*}
 done
 
 
@@ -244,26 +239,25 @@ lemma Spy_not_see_encrypted_key:
 by (blast dest: Says_Server_message_form secrecy_lemma)
 
 
-(*** Attempting to prove stronger properties ***)
+subsection{*Attempting to prove stronger properties *}
 
-(*Only OR1 can have caused such a part of a message to appear.
-  The premise A \<noteq> B prevents OR2's similar-looking cryptogram from being
-  picked up.  Original Otway-Rees doesn't need it.*)
+text{*Only OR1 can have caused such a part of a message to appear. The premise
+  @{term "A \<noteq> B"} prevents OR2's similar-looking cryptogram from being picked 
+  up. Original Otway-Rees doesn't need it.*}
 lemma Crypt_imp_OR1 [rule_format]:
      "[| A \<notin> bad;  A \<noteq> B;  evs \<in> otway |]
       ==> Crypt (shrK A) {|NA, Agent A, Agent B|} \<in> parts (knows Spy evs) -->
           Says A B {|NA, Agent A, Agent B,
                      Crypt (shrK A) {|NA, Agent A, Agent B|}|}  \<in> set evs"
-apply (erule otway.induct, force,
-       drule_tac [4] OR2_parts_knows_Spy, simp_all, blast+)
-done
+by (erule otway.induct, force,
+    drule_tac [4] OR2_parts_knows_Spy, simp_all, blast+)
 
 
-(*Crucial property: If the encrypted message appears, and A has used NA
+text{*Crucial property: If the encrypted message appears, and A has used NA
   to start a run, then it originated with the Server!
-  The premise A \<noteq> B allows use of Crypt_imp_OR1*)
-(*Only it is FALSE.  Somebody could make a fake message to Server
-          substituting some other nonce NA' for NB.*)
+  The premise @{term "A \<noteq> B"} allows use of @{text Crypt_imp_OR1}*}
+text{*Only it is FALSE.  Somebody could make a fake message to Server
+          substituting some other nonce NA' for NB.*}
 lemma "[| A \<notin> bad;  A \<noteq> B;  evs \<in> otway |]
        ==> Crypt (shrK A) {|NA, Key K|} \<in> parts (knows Spy evs) -->
            Says A B {|NA, Agent A, Agent B,
@@ -275,15 +269,12 @@ lemma "[| A \<notin> bad;  A \<noteq> B;  evs \<in> otway |]
                   Crypt (shrK B) {|NB, Key K|}|}  \<in> set evs)"
 apply (erule otway.induct, force,
        drule_tac [4] OR2_parts_knows_Spy, simp_all)
-(*Fake*)
-apply blast
-(*OR1: it cannot be a new Nonce, contradiction.*)
-apply blast
-(*OR3 and OR4*)
+apply blast  --{*Fake*}
+apply blast  --{*OR1: it cannot be a new Nonce, contradiction.*}
+txt{*OR3 and OR4*}
 apply (simp_all add: ex_disj_distrib)
-(*OR4*)
-prefer 2 apply (blast intro!: Crypt_imp_OR1)
-(*OR3*)
+ prefer 2 apply (blast intro!: Crypt_imp_OR1)  --{*OR4*}
+txt{*OR3*}
 apply clarify
 (*The hypotheses at this point suggest an attack in which nonce NB is used
   in two different roles:
